FCtx attempt...

FreydSSA/Term/Extrinsic/Subst.lean
@@ -1,5 +1,7 @@
 import FreydSSA.Term.Extrinsic.Basic
 
+variable {φ ν α} [Φ : InstSet φ (Ty α)] [Φc : CohInstSet φ (Ty α)]
+
 inductive InstSet.USubst [Φ : InstSet φ (Ty α)] (σ : ν → UTm φ ν)
   : Ctx ν (Ty α) → Ctx ν (Ty α) → Type _
 | nil (Γ) : Φ.USubst σ Γ []
@@ -8,18 +10,18 @@ inductive InstSet.USubst [Φ : InstSet φ (Ty α)] (σ : ν → UTm φ ν)
   Φ.USubst σ Γ Δ →
   Φ.USubst σ Γ (⟨x, A⟩::Δ)
 
-def InstSet.USubst.fromTuple [Φ : InstSet φ (Ty α)] {Γ Δ : Ctx ν (Ty α)}
+def InstSet.USubst.fromTuple {Γ Δ : Ctx ν (Ty α)}
   (f: (i : Fin Δ.length) → (σ (Δ.get i).name).Wf 1 Γ (Δ.get i).ty) : Φ.USubst σ Γ Δ
   := match Δ with
   | [] => nil _
   | v::Δ => cons (f ⟨0, by simp⟩) (fromTuple (λi => f i.succ))
 
-def InstSet.USubst.get [Φ : InstSet φ (Ty α)] {Γ Δ : Ctx ν (Ty α)}
+def InstSet.USubst.get {Γ Δ : Ctx ν (Ty α)}
   : Φ.USubst σ Γ Δ → (i : Fin Δ.length) → (σ (Δ.get i).name).Wf 1 Γ (Δ.get i).ty
   | cons e _, ⟨0, _⟩ => e
   | cons _ σ, ⟨n + 1, hn⟩ => σ.get ⟨n, Nat.lt_of_succ_lt_succ hn⟩
 
-theorem InstSet.USubst.fromTuple_get [Φ : InstSet φ (Ty α)] {Γ Δ : Ctx ν (Ty α)}
+theorem InstSet.USubst.fromTuple_get {Γ Δ : Ctx ν (Ty α)}
   : (hσ : Φ.USubst σ Γ Δ) → fromTuple (hσ.get) = hσ
   | nil _ => rfl
   | cons e hσ => by
@@ -30,7 +32,7 @@ theorem InstSet.USubst.fromTuple_get [Φ : InstSet φ (Ty α)] {Γ Δ : Ctx ν (
     rw [fromTuple_get hσ]
     rfl
 
-theorem InstSet.USubst.get_fromTuple [Φ : InstSet φ (Ty α)] {Γ Δ : Ctx ν (Ty α)}
+theorem InstSet.USubst.get_fromTuple {Γ Δ : Ctx ν (Ty α)}
   {σ : ν → UTm φ ν}
   (hσ : (i : Fin Δ.length) → (σ (Δ.get i).name).Wf 1 Γ (Δ.get i).ty) : get (fromTuple hσ) = hσ
   := by induction Δ with
@@ -39,18 +41,18 @@ theorem InstSet.USubst.get_fromTuple [Φ : InstSet φ (Ty α)] {Γ Δ : Ctx ν (
     funext ⟨i, hi⟩
     cases i <;> simp only [fromTuple, get, Fin.succ, *]
 
-def InstSet.USubst.wk_entry [Φ : InstSet φ (Ty α)] {Γ Γ' Δ : Ctx ν (Ty α)} {σ}
+def InstSet.USubst.wk_entry {Γ Γ' Δ : Ctx ν (Ty α)} {σ}
   : Γ'.Wk Γ → Φ.USubst σ Γ Δ → Φ.USubst σ Γ' Δ
   | _, nil _ => nil _
   | w, cons e hσ => cons (e.wk w) (wk_entry w hσ)
 
-def InstSet.USubst.wk_exit [Φ : InstSet φ (Ty α)] {Γ Δ Δ' : Ctx ν (Ty α)} {σ}
+def InstSet.USubst.wk_exit {Γ Δ Δ' : Ctx ν (Ty α)} {σ}
   : Φ.USubst σ Γ Δ → Δ.Wk Δ' → Φ.USubst σ Γ Δ'
   | nil _, Ctx.Wk.nil => nil _
   | cons _ hσ, Ctx.Wk.skip _ w => hσ.wk_exit w
   | cons e hσ, Ctx.Wk.cons _ w => cons e (hσ.wk_exit w)
 
-def InstSet.USubst.tensor [Φ : InstSet φ (Ty α)] {Γ Δ : Ctx ν (Ty α)} {σ}
+def InstSet.USubst.tensor {Γ Δ : Ctx ν (Ty α)} {σ}
   (hx : x.name ∉ Γ.names)
   (hx' : σ x.name = UTm.var x.name)
   (hσ : Φ.USubst σ Γ Δ) : Φ.USubst σ (x::Γ) (x::Δ)
@@ -58,10 +60,16 @@ def InstSet.USubst.tensor [Φ : InstSet φ (Ty α)] {Γ Δ : Ctx ν (Ty α)} {σ
     (hx' ▸ (UTm.Wf.var _ (Ctx.Wk.head _ _)))
     (hσ.wk_entry (Ctx.Wk.skip (Ctx.Fresh.of_not_mem_names hx) (Ctx.Wk.refl _)))
 
-def UTm.Wf.subst [Φ : InstSet φ (Ty α)] {σ : ν → UTm φ ν} {Γ Δ : Ctx ν (Ty α)}
+def UTm.Wf.subst {σ : ν → UTm φ ν} {Γ Δ : Ctx ν (Ty α)}
   {e : UTm φ ν} (hσ : Φ.USubst σ Γ Δ) : e.Wf p Δ A → (e.rewrite σ).Wf p Γ A
   | var x w => match hσ.wk_exit w with | InstSet.USubst.cons e _ => e.of_pure
   | op f e => op f (e.subst hσ)
   | pair p l r => pair p (l.subst hσ) (r.subst hσ)
   | unit p => unit p
   | bool p b => bool p b
+
+def InstSet.USubst.wk_meet {Γ₁ Γ₂ Γ Δ : Ctx ν (Ty α)} {σ}
+  (w : Γ.Wk Γ₁) (w' : Γ.Wk Γ₂)
+  : Φ.USubst σ Γ₁ Δ → Φ.USubst σ Γ₂ Δ → Φ.USubst σ (w.meet w') Δ
+  | nil _, nil _ => nil _
+  | cons e hσ, cons e' hσ' => cons (e.wk_meet w w' e') (wk_meet w w' hσ hσ')
