FreydSSA/FCtx.lean
@@ -1,0 +1,149 @@
+import Mathlib.Data.List.Basic
+import Mathlib.Data.List.MinMax
+import Mathlib.Data.List.Nodup
+import Mathlib.Data.Set.Basic
+import Mathlib.Data.Set.Function
+import Mathlib.Data.Set.Finite
+import Mathlib.Data.Fin.Basic
+import Mathlib.Init.Classical
+import Mathlib.Order.SuccPred.Basic
+
+variable {ν ν' α β} [DecidableEq ν] [DecidableEq ν']
+
+structure FCtx (ν : Type u) (α : Type v) : Type (max u v) where
+  toFun : ν → WithBot α
+  support : Finset ν
+  mem_support_toFun : ∀x, x ∈ support ↔ toFun x ≠ ⊥
+
+theorem FCtx.ext {Γ Δ : FCtx ν α} (h : Γ.toFun = Δ.toFun)
+  : Γ = Δ
+  := match Γ, Δ with
+  | ⟨fΓ, n, hm⟩, ⟨fΔ, n', hm'⟩ => by
+    cases h
+    simp only [mk.injEq, true_and]
+    apply Finset.ext
+    intro x
+    rw [hm, hm']
+
+theorem FCtx.ext_iff {Γ Δ : FCtx ν α}
+  : Γ = Δ ↔ Γ.toFun = Δ.toFun
+  := ⟨(λh => by cases h; rfl), FCtx.ext⟩
+
+instance FCtx.instFunLike : FunLike (FCtx ν α) ν (WithBot α) where
+  coe := FCtx.toFun
+  coe_injective' := by intro Γ Δ; apply FCtx.ext
+
+def FCtx.map_ty (Γ : FCtx ν α) (f : α → β) : FCtx ν β where
+  toFun x := (Γ.toFun x).map (f)
+  support := Γ.support
+  mem_support_toFun := by
+    intro x
+    rw [Γ.mem_support_toFun x]
+    simp only []
+    generalize Γ.toFun x = a
+    cases a <;> simp [WithBot.map, Bot.bot]
+
+def FCtx.cons (x : ν) (a : α) (Γ : FCtx ν α) : FCtx ν α where
+  toFun := Function.update Γ.toFun x a
+  support := Γ.support ∪ {x}
+  mem_support_toFun := by
+    intro y
+    simp only [Finset.mem_union, Function.update]
+    split <;> simp [*, mem_support_toFun]
+
+def FCtx.cons_inj {x : ν} {a a' : α} {Γ : FCtx ν α}
+  (h : Γ.cons x a = Γ.cons x a') : a = a' :=
+  have hl : Γ.cons x a x = a := by simp [FCtx.cons, DFunLike.coe]
+  have hr : Γ.cons x a' x = a' := by simp [FCtx.cons, DFunLike.coe]
+  by rw [<-WithBot.coe_inj, <-hl, <-hr, h]
+
+def FCtx.Wk (Γ Δ : FCtx ν α) : Prop := ∀x, Δ.toFun x = ⊥ ∨ Δ.toFun x = Γ.toFun x
+
+theorem FCtx.Wk.refl (Γ : FCtx ν α) : FCtx.Wk Γ Γ := by simp [FCtx.Wk]
+theorem FCtx.Wk.trans {Γ Δ Θ : FCtx ν α} (w : FCtx.Wk Γ Δ) (w' : FCtx.Wk Δ Θ)
+  : FCtx.Wk Γ Θ := by
+  intro x
+  cases w x <;> cases w' x <;> simp [*]
+theorem FCtx.Wk.antisymm {Γ Δ : FCtx ν α} (w : FCtx.Wk Γ Δ) (w' : FCtx.Wk Δ Γ)
+  : Γ = Δ := by
+  apply FCtx.ext
+  funext x
+  cases w x with
+  | inl h => cases w' x with | inl h' => rw [h, h'] | inr h' => exact h'
+  | inr h => exact h.symm
+
+def FCtx.Wk.src {Γ Δ : FCtx ν α} (_ : FCtx.Wk Γ Δ) : FCtx ν α := Γ
+def FCtx.Wk.trg {Γ Δ : FCtx ν α} (_ : FCtx.Wk Γ Δ) : FCtx ν α := Δ
+
+theorem FCtx.Wk.eq_bot {Γ Δ : FCtx ν α} (w : FCtx.Wk Γ Δ) (x : ν) (h : Γ.toFun x = ⊥)
+  : Δ.toFun x = ⊥ := by cases w x <;> simp [*]
+theorem FCtx.Wk.ne_bot {Γ Δ : FCtx ν α} (w : FCtx.Wk Γ Δ) (x : ν) (h : Δ.toFun x ≠ ⊥)
+  : Γ.toFun x ≠ ⊥ := λh' => h (w.eq_bot _ h')
+theorem FCtx.Wk.eq_some_ne_bot {Γ Δ : FCtx ν α} (w : FCtx.Wk Γ Δ)
+  (x : ν) (h : Δ.toFun x ≠ ⊥)
+  : Γ.toFun x ≠ ⊥ := λh' => h (w.eq_bot _ h')
+
+theorem FCtx.Wk.support_subset {Γ Δ : FCtx ν α} (w : FCtx.Wk Γ Δ)
+  : Δ.support ⊆ Γ.support := by
+  intro x
+  rw [Γ.mem_support_toFun, Δ.mem_support_toFun]
+  exact w.ne_bot x
+
+instance FCtx.instPartialOrder : PartialOrder (FCtx ν α) where
+  le := FCtx.Wk
+  le_refl := FCtx.Wk.refl
+  le_trans _ _ _ := FCtx.Wk.trans
+  le_antisymm _ _ := FCtx.Wk.antisymm
+
+def FCtx.linf (Δ Δ' : FCtx ν α)
+  : FCtx ν α where
+  toFun x := match Δ.toFun x, Δ'.toFun x with
+    | ⊥, _ | _, ⊥ => ⊥
+    | some a, some _ => some a
+  support := Δ.support ∩ Δ'.support
+  mem_support_toFun := by
+    intro x
+    simp only [Finset.mem_inter, mem_support_toFun]
+    split <;> simp [Bot.bot, *]
+
+def FCtx.rinf (Δ Δ' : FCtx ν α)
+  : FCtx ν α where
+  toFun x := match Δ.toFun x, Δ'.toFun x with
+    | ⊥, _ | _, ⊥ => ⊥
+    | some _, some a => some a
+  support := Δ.support ∩ Δ'.support
+  mem_support_toFun := by
+    intro x
+    simp only [Finset.mem_inter, mem_support_toFun]
+    split <;> simp [Bot.bot, *]
+
+theorem FCtx.Wk.var_eq {Γ Δ : FCtx ν α} (w : FCtx.Wk Γ Δ) (x : ν) (a b : α)
+  (h : Γ.toFun x = a) (h' : Δ.toFun x = b)
+  : a = b := by
+  cases w x
+  case inl hw => rw [hw] at h'; cases h'
+  case inr hw => rw [hw] at h'; rw [h'] at h; cases h; rfl
+
+theorem FCtx.Wk.var {Γ Δ : FCtx ν α} (w : FCtx.Wk Γ Δ) (x : ν) (a : α)
+  (h : Δ.toFun x = a) : Γ.toFun x = a := by
+  cases w x
+  case inl hw => rw [hw] at h; cases h
+  case inr hw => rw [hw] at h; exact h
+
+def FCtx.Wk.var_eq₂' {Γ Δ Δ' : FCtx ν α} (w : FCtx.Wk Γ Δ) (w' : FCtx.Wk Γ Δ')
+  (x : ν) (a b : α) (h : Δ.toFun x = a) (h' : Δ'.toFun x = b)
+  : (a : WithBot α) = (b : WithBot α) := by rw [<-var w x a h, <-var w' x b h']
+
+def FCtx.Wk.var_eq₂ {Γ Δ Δ' : FCtx ν α} (w : FCtx.Wk Γ Δ) (w' : FCtx.Wk Γ Δ')
+  (x : ν) (a b : α) (h : Δ.toFun x = a) (h' : Δ'.toFun x = b)
+  : a = b := by cases var_eq₂' w w' x a b h h'; rfl
+
+def FCtx.Wk.linf_eq_rinf {Γ Δ Δ' : FCtx ν α} (w : FCtx.Wk Γ Δ) (w' : FCtx.Wk Γ Δ')
+  : FCtx.linf Δ Δ' = FCtx.rinf Δ Δ' := by
+  apply FCtx.ext
+  funext x
+  simp only [linf, rinf]
+  split
+  . rfl
+  . rfl
+  . apply var_eq₂' w w' <;> assumption
