FreydSSA/Term/Extrinsic/Basic.lean
@@ -49,18 +49,18 @@ def UTm.Wf.wk {e : UTm φ ν} (w : Γ.Wk Δ) : e.Wf p Δ A → e.Wf p Γ A
   | unit p => unit p
   | bool p b => bool p b
 
--- def UTm.Wf.wk_meet {e : UTm φ ν}
---   (w : Γ.Wk Δ) (w' : Γ.Wk Δ') : e.Wf p Δ A → e.Wf p Δ' A → e.Wf p (w.meet w') A
---   | var _ w, var _ w' => var p sorry --TODO: meet must actually _be_ a meet...
---   | op hf de, op hf' de' => by
---     cases (de.wk w).tyEq (de'.wk w')
---     exact op hf (de.wk_meet w w' de')
---   | pair _ dl dr, pair _ dl' dr' => by
---     cases (dl.wk w).tyEq (dl'.wk w')
---     cases (dr.wk w).tyEq (dr'.wk w')
---     exact pair p (dl.wk_meet w w' dl') (dr.wk_meet w w' dr')
---   | unit _, unit _ => unit p
---   | bool _ _, bool _ b => bool p b
+def UTm.Wf.wk_meet {e : UTm φ ν}
+  (w : Γ.Wk Δ) (w' : Γ.Wk Δ') : e.Wf p Δ A → e.Wf p Δ' A → e.Wf p (w.meet w') A
+  | var _ i, var _ i' => var p (w.meet_var w' i i')
+  | op hf de, op hf' de' => by
+    cases (de.wk w).tyEq (de'.wk w')
+    exact op hf (de.wk_meet w w' de')
+  | pair _ dl dr, pair _ dl' dr' => by
+    cases (dl.wk w).tyEq (dl'.wk w')
+    cases (dr.wk w).tyEq (dr'.wk w')
+    exact pair p (dl.wk_meet w w' dl') (dr.wk_meet w w' dr')
+  | unit _, unit _ => unit p
+  | bool _ _, bool _ b => bool p b
 
 inductive UTm.Wf.Iso {Γ' : Ctx ν' (Ty α)}
   : {e : UTm φ ν} → {e' : UTm φ ν'} → e.Wf p Γ A → e'.Wf p Γ' A → Prop
